

1 Gauge-Invariance

Let

$$\dot{x} = Ax, y = Cx + b, \dot{b} = 0$$

be given. The bias term is modeled as,

$$b \triangleq \alpha C + \beta C^\perp$$

where $C^T C^\perp = (C^\perp)^T C = 0$ or alternatively $C \perp C^\perp$, and the projection matrix is chosen as,

$$\Pi \triangleq I - \frac{CC^T}{C^T C}$$

The following can be stated,

$$\begin{aligned}\Pi C &= \left(I - \frac{CC^T}{C^T C} \right) C \\ &= C - \frac{CC^T C}{C^T C} \\ &= C - C \\ \Pi C &= 0\end{aligned}$$

and

$$\begin{aligned}\Pi C^\perp &= \left(I - \frac{CC^T}{C^T C} \right) C^\perp \\ &= C^\perp - \frac{CC^T C^\perp}{C^T C} \\ \Pi C^\perp &= C^\perp\end{aligned}$$

The projection matrix applied on the bias Πb gives,

$$\begin{aligned}\Pi b &= \Pi(\alpha C + \beta C^\perp) \\ &= \alpha \Pi C + \beta \Pi C^\perp \\ &= \beta C^\perp\end{aligned}$$

Π applied to the output gives,

$$\begin{aligned}\Pi y &= \Pi(Cx + \alpha C + \beta C^\perp) \\ &= \Pi Cx + \alpha \Pi C + \beta \Pi C^\perp \\ &= \beta \Pi C^\perp \\ &= \beta C^\perp\end{aligned}$$

and β can be recovered using,

$$\begin{aligned}(C^\perp)^T(\Pi y) &= \beta C^\perp \\ (C^\perp)^T \Pi y &= (C^\perp)^T \beta C^\perp \\ (C^\perp)^T \Pi y &= \beta (C^\perp)^T C^\perp \\ \beta &= \frac{(C^\perp)^T \Pi y}{(C^\perp)^T C^\perp}\end{aligned}$$

Here, the bias perpendicular to the output vector C can be recovered but, the bias aligned with the output can not be recovered via the projection. This can also be observed by the following,

$$\begin{aligned}\dot{x} &= Ax, y = Cx + b, \dot{b} = 0 \\ \dot{x} &= Ax, y = Cx + \alpha C + \beta C^\perp, \alpha \dot{C} + \dot{\beta} C^\perp = 0 \\ \dot{x} &= Ax, y = C(x + \alpha) + \beta C^\perp, \dot{\alpha} C + \dot{\beta} C^\perp = 0 \\ \dot{x} &= Ax, y = C(x + \alpha) + \beta C^\perp, \dot{\alpha} = 0, \dot{\beta} = 0\end{aligned}$$

Defining $z \triangleq x + \alpha$,

$$\dot{z} = Az - \alpha A, y = Cz + \beta C^\perp, \dot{\alpha} = 0, \dot{\beta} = 0$$

gives

$$\begin{bmatrix} \dot{z} \\ \dot{\alpha} \end{bmatrix} = \begin{bmatrix} A & -A \\ 0 & 0 \end{bmatrix} \begin{bmatrix} z \\ \alpha \end{bmatrix}, y = [C \quad 0] \begin{bmatrix} z \\ \alpha \end{bmatrix} + \beta C^\perp, x = [I \quad -I] \begin{bmatrix} z \\ \alpha \end{bmatrix}$$

An observer as follows,

$$\begin{bmatrix} \dot{\hat{z}} \\ \dot{\hat{\alpha}} \end{bmatrix} = \begin{bmatrix} A & -A \\ 0 & 0 \end{bmatrix} \begin{bmatrix} \hat{z} \\ \hat{\alpha} \end{bmatrix} + \begin{bmatrix} L \\ L_\alpha \end{bmatrix} (y - \hat{y}), \hat{y} = [C \quad 0] \begin{bmatrix} \hat{z} \\ \hat{\alpha} \end{bmatrix} + \Pi y, \hat{x} = [I \quad -I] \begin{bmatrix} \hat{z} \\ \hat{\alpha} \end{bmatrix}$$

may be used to determine x and α where β is obtained using the projection.